src/kernel/quot.cpp
@@ -20,25 +20,32 @@ static void check_eq_type(environment const & env) {
     constant_info eq_info = env.get("Eq");
     if (!eq_info.is_inductive()) throw exception("failed to initialize quot module, environment does not have 'Eq' type");
     inductive_val eq_val  = eq_info.to_inductive_val();
-    if (length(eq_info.get_lparams()) != 1)
+    if (length(eq_info.get_lparams()) != 2)
         throw exception("failed to initialize quot module, unexpected number of universe params at 'Eq' type");
     if (length(eq_val.get_cnstrs()) != 1)
         throw exception("failed to initialize quot module, unexpected number of constructors for 'Eq' type");
     local_ctx lctx;
     name_generator g;
     {
-        level u = mk_univ_param(head(eq_info.get_lparams()));
-        expr alpha = lctx.mk_local_decl(g, "α", mk_sort(u), mk_implicit_binder_info());
-        expr expected_eq_type = lctx.mk_pi(alpha, mk_arrow(alpha, mk_arrow(alpha, mk_Prop())));
+        names lps = eq_info.get_lparams();
+        level u = mk_univ_param(head(lps));
+        level h = mk_univ_param(head(tail(lps)));
+        expr alpha = lctx.mk_local_decl(g, "α", mk_sort(u, h), mk_implicit_binder_info());
+        expr Prop_h = mk_sort(mk_level_zero(), h);
+        expr expected_eq_type = lctx.mk_pi(alpha, mk_arrow(alpha, mk_arrow(alpha, Prop_h)));
         if (expected_eq_type != eq_info.get_type())
             throw exception("failed to initialize quot module, 'Eq' has an expected type");
     }
     {
         constant_info eq_refl_info = env.get(head(eq_val.get_cnstrs()));
-        level u = mk_univ_param(head(eq_refl_info.get_lparams()));
-        expr alpha = lctx.mk_local_decl(g, "α", mk_sort(u), mk_implicit_binder_info());
+        if (length(eq_refl_info.get_lparams()) != 2)
+            throw exception("failed to initialize quot module, unexpected number of universe params at 'Eq.refl' constructor");
+        names lps = eq_refl_info.get_lparams();
+        level u = mk_univ_param(head(lps));
+        level h = mk_univ_param(head(tail(lps)));
+        expr alpha = lctx.mk_local_decl(g, "α", mk_sort(u, h), mk_implicit_binder_info());
         expr a = lctx.mk_local_decl(g, "a", alpha);
-        expr expected_eq_refl_type = lctx.mk_pi({alpha, a}, mk_app(mk_constant("Eq", {u}), alpha, a, a));
+        expr expected_eq_refl_type = lctx.mk_pi({alpha, a}, mk_app(mk_constant("Eq", {u, h}), alpha, a, a));
         if (eq_refl_info.get_type() != expected_eq_refl_type)
             throw exception("failed to initialize quot module, unexpected type for 'Eq' type constructor");
     }
@@ -50,48 +57,51 @@ environment environment::add_quot() const {
     check_eq_type(*this);
     environment new_env = *this;
     name u_name("u");
+    name h_name("h");
     local_ctx lctx;
     name_generator g;
     level u         = mk_univ_param(u_name);
-    expr Sort_u     = mk_sort(u);
+    level h         = mk_univ_param(h_name);
+    expr Sort_u     = mk_sort(u, h);
+    expr Prop_h     = mk_sort(mk_level_zero(), h);
     expr alpha      = lctx.mk_local_decl(g, "α", Sort_u, mk_implicit_binder_info());
-    expr r          = lctx.mk_local_decl(g, "r", mk_arrow(alpha, mk_arrow(alpha, mk_Prop())));
-    /* constant {u} quot {α : Sort u} (r : α → α → Prop) : Sort u */
-    new_env.add_core(constant_info(quot_val(*quot_consts::g_quot, {u_name}, lctx.mk_pi({alpha, r}, Sort_u), quot_kind::Type)));
-    expr quot_r     = mk_app(mk_constant(*quot_consts::g_quot, {u}), alpha, r);
+    expr r          = lctx.mk_local_decl(g, "r", mk_arrow(alpha, mk_arrow(alpha, Prop_h)));
+    /* constant {u h} quot {α : Sort u @ h} (r : α → α → Prop @ h) : Sort u @ h */
+    new_env.add_core(constant_info(quot_val(*quot_consts::g_quot, {u_name, h_name}, lctx.mk_pi({alpha, r}, Sort_u), quot_kind::Type)));
+    expr quot_r     = mk_app(mk_constant(*quot_consts::g_quot, {u, h}), alpha, r);
     expr a          = lctx.mk_local_decl(g, "a", alpha);
-    /* constant {u} quot.mk {α : Sort u} (r : α → α → Prop) (a : α) : @quot.{u} α r */
-    new_env.add_core(constant_info(quot_val(*quot_consts::g_quot_mk, {u_name}, lctx.mk_pi({alpha, r, a}, quot_r), quot_kind::Mk)));
+    /* constant {u h} quot.mk {α : Sort u @ h} (r : α → α → Prop @ h) (a : α) : @quot.{u,h} α r */
+    new_env.add_core(constant_info(quot_val(*quot_consts::g_quot_mk, {u_name, h_name}, lctx.mk_pi({alpha, r, a}, quot_r), quot_kind::Mk)));
     /* make r implicit */
     lctx = local_ctx();
     alpha           = lctx.mk_local_decl(g, "α", Sort_u, mk_implicit_binder_info());
-    r               = lctx.mk_local_decl(g, "r", mk_arrow(alpha, mk_arrow(alpha, mk_Prop())), mk_implicit_binder_info());
-    quot_r          = mk_app(mk_constant(*quot_consts::g_quot, {u}), alpha, r);
+    r               = lctx.mk_local_decl(g, "r", mk_arrow(alpha, mk_arrow(alpha, Prop_h)), mk_implicit_binder_info());
+    quot_r          = mk_app(mk_constant(*quot_consts::g_quot, {u, h}), alpha, r);
     a               = lctx.mk_local_decl(g, "a", alpha);
     name v_name("v");
     level v         = mk_univ_param(v_name);
-    expr Sort_v     = mk_sort(v);
+    expr Sort_v     = mk_sort(v, h);
     expr beta       = lctx.mk_local_decl(g, "β", Sort_v, mk_implicit_binder_info());
     expr f          = lctx.mk_local_decl(g, "f", mk_arrow(alpha, beta));
     expr b          = lctx.mk_local_decl(g, "b", alpha);
     expr r_a_b      = mk_app(r, a, b);
     /* f a = f b */
-    expr f_a_eq_f_b = mk_app(mk_constant("Eq", {v}), beta, mk_app(f, a), mk_app(f, b));
+    expr f_a_eq_f_b = mk_app(mk_constant("Eq", {v, h}), beta, mk_app(f, a), mk_app(f, b));
     /* (∀ a b : α, r a b → f a = f b) */
     expr sanity     = lctx.mk_pi({a, b}, mk_arrow(r_a_b, f_a_eq_f_b));
-    /* constant {u v} quot.lift {α : Sort u} {r : α → α → Prop} {β : Sort v} (f : α → β)
-                                : (∀ a b : α, r a b → f a = f b) →  @quot.{u} α r → β */
-    new_env.add_core(constant_info(quot_val(*quot_consts::g_quot_lift, {u_name, v_name},
+    /* constant {u v h} quot.lift {α : Sort u @ h} {r : α → α → Prop @ h} {β : Sort v @ h} (f : α → β)
+                                : (∀ a b : α, r a b → f a = f b) →  @quot.{u,h} α r → β */
+    new_env.add_core(constant_info(quot_val(*quot_consts::g_quot_lift, {u_name, v_name, h_name},
                                             lctx.mk_pi({alpha, r, beta, f}, mk_arrow(sanity, mk_arrow(quot_r, beta))), quot_kind::Lift)));
-    /* {β : @quot.{u} α r → Prop} */
-    beta            = lctx.mk_local_decl(g, "β", mk_arrow(quot_r, mk_Prop()), mk_implicit_binder_info());
-    expr quot_mk_a  = mk_app(mk_constant(*quot_consts::g_quot_mk, {u}), alpha, r, a);
+    /* {β : @quot.{u,h} α r → Prop @ h} */
+    beta            = lctx.mk_local_decl(g, "β", mk_arrow(quot_r, Prop_h), mk_implicit_binder_info());
+    expr quot_mk_a  = mk_app(mk_constant(*quot_consts::g_quot_mk, {u, h}), alpha, r, a);
     expr all_quot   = lctx.mk_pi(a, mk_app(beta, quot_mk_a));
     expr q          = lctx.mk_local_decl(g, "q", quot_r);
     expr beta_q     = mk_app(beta, q);
-    /* constant {u} quot.ind {α : Sort u} {r : α → α → Prop} {β : @quot.{u} α r → Prop}
-                   : (∀ a : α, β (@quot.mk.{u} α r a)) → ∀ q : @quot.{u} α r, β q */
-    new_env.add_core(constant_info(quot_val(*quot_consts::g_quot_ind, {u_name},
+    /* constant {u h} quot.ind {α : Sort u @ h} {r : α → α → Prop @ h} {β : @quot.{u,h} α r → Prop @ h}
+                   : (∀ a : α, β (@quot.mk.{u,h} α r a)) → ∀ q : @quot.{u,h} α r, β q */
+    new_env.add_core(constant_info(quot_val(*quot_consts::g_quot_ind, {u_name, h_name},
                                             lctx.mk_pi({alpha, r, beta}, mk_pi("mk", all_quot, lctx.mk_pi(q, beta_q))), quot_kind::Ind)));
     new_env.mark_quot_initialized();
     return new_env;
